extraction/theories/Aux.v
@@ -10,22 +10,24 @@ Ltac propify :=
   unfold is_true in *;
   repeat
     match goal with
-    | [H: context[orb _ _ = false] |- _] => rewrite Bool.orb_false_iff in H
-    | [H: context[orb _ _ = true] |- _] => rewrite Bool.orb_true_iff in H
-    | [|- context[orb _ _ = false]] => rewrite Bool.orb_false_iff
-    | [|- context[orb _ _ = true]] => rewrite Bool.orb_true_iff
+    | [H: context[Nat.eqb _ _ = false] |- _] => rewrite Nat.eqb_neq in H
+    | [H: context[Nat.eqb _ _ = true] |- _] => rewrite Nat.eqb_eq in H
+    | [H: context[Nat.ltb _ _ = false] |- _] => rewrite Nat.ltb_ge in H
+    | [H: context[Nat.ltb _ _ = true] |- _] => rewrite Nat.ltb_lt in H
     | [H: context[andb _ _ = false] |- _] => rewrite Bool.andb_false_iff in H
     | [H: context[andb _ _ = true] |- _] => rewrite Bool.andb_true_iff in H
-    | [H: context[negb _ = true] |- _] => rewrite Bool.negb_true_iff in H
     | [H: context[negb _ = false] |- _] => rewrite Bool.negb_false_iff in H
+    | [H: context[negb _ = true] |- _] => rewrite Bool.negb_true_iff in H
+    | [H: context[orb _ _ = false] |- _] => rewrite Bool.orb_false_iff in H
+    | [H: context[orb _ _ = true] |- _] => rewrite Bool.orb_true_iff in H
+    | [|- context[Nat.eqb _ _ = false]] => rewrite Nat.eqb_neq
+    | [|- context[Nat.eqb _ _ = true]] => rewrite Nat.eqb_eq
+    | [|- context[Nat.ltb _ _ = false]] => rewrite Nat.ltb_ge
+    | [|- context[Nat.ltb _ _ = true]] => rewrite Nat.ltb_lt
     | [|- context[andb _ _ = false]] => rewrite Bool.andb_false_iff
     | [|- context[andb _ _ = true]] => rewrite Bool.andb_true_iff
-    | [H: context[Nat.ltb _ _ = true] |- _] => rewrite Nat.ltb_lt in H
-    | [H: context[Nat.ltb _ _ = false] |- _] => rewrite Nat.ltb_ge in H
-    | [|- context[Nat.ltb _ _ = true]] => rewrite Nat.ltb_lt
-    | [|- context[Nat.ltb _ _ = false]] => rewrite Nat.ltb_ge
-    | [H: context[Nat.eqb _ _ = true] |- _] => rewrite Nat.eqb_eq in H
-    | [H: context[Nat.eqb _ _ = false] |- _] => rewrite Nat.eqb_neq in H
-    | [|- context[Nat.eqb _ _ = true]] => rewrite Nat.eqb_eq
-    | [|- context[Nat.eqb _ _ = false]] => rewrite Nat.eqb_neq
+    | [|- context[negb _ = false]] => rewrite Bool.negb_false_iff
+    | [|- context[negb _ = true]] => rewrite Bool.negb_true_iff
+    | [|- context[orb _ _ = false]] => rewrite Bool.orb_false_iff
+    | [|- context[orb _ _ = true]] => rewrite Bool.orb_true_iff
     end.
